\problem{A2}

Let $F_i$ be the fibonacci numbers.
Use complete induction to prove that $F_n \geq \alpha^{n - 2}$ for all $n \geq 1$ where $\alpha = (1 + \sqrt{5})/2$.

\solution

\part 

\begin{theorem}
The formula $F_n \geq \alpha^{nâˆ’2}$ is true for all $n \geq 1$ where $\alpha = (1 + \sqrt{5})/2$.
\end{theorem}

\begin{proof}
First consider the base cases $n = 1$ and $n = 2$. First, $F_1 = 1$ and $F_2 = 2$. 
For $n = 1$, $\alpha^{n - 2} = \frac{2}{\sqrt{5} + 1} = 0.618..$, which is less than $1$.
For $n = 2$, $\alpha^{n - 2} = 1$, which is less than $2$.
Now, suppose that for all $k$ in  $n \geq k \geq 1$, $F_k \geq \alpha^{n - 2}$.
% By the formula of the fibonacci numbers, $F_{n + 1} = F_n + F_{n - 1}$.
% From this, it must be shown that $F_n + F_{n -1} \geq \alpha_{n - 2}$.
Using the induction hypothesis and the formula for the fibonacci numbers, $F_{n + 1} = F_n + F_{n - 1} \geq \alpha^{n - 2} + \alpha^{n - 3}$. 
Consider $\alpha = (1 + \sqrt{5}/2)$. $\alpha^2 = \frac{6 + 2*\sqrt{5}}{4} = \frac{2 + 1 + \sqrt{5}/2} = 1 + \alpha$.
From above we can now say $F_{n + 1} \geq \alpha^{n - 3} * (\alpha + 1) = \alpha{n - 3} * \alpha^2 = \alpha{n - 1}$.
Thus, since $F_{n + 1} \geq \alpha{n - 1}$, by the principle of complete mathematical induction, the hypothesis holds.
\end{proof}
