\problem{Direct Proof}

Use a direct proof to prove that ``If x + y is even and y + z is even, then x + z is even''.

\solution

\part 

\begin{theorem}
If x + y is even and y + z is even, then x + z is even.
\end{theorem}
\begin{proof}
The definition of an even number is that the number is divisible by two such that $n = 2a$.
By this definition, $x + y = 2a$ and $y + z = 2b$.
So $x + y + y + z = 2a + 2b$, which simplifies to $x + z = 2(a + b - y)$.
Since $a + b - y$ is just an integer (call it $c$), then $x + z = 2c$ and therefore $x + z$ is even.
\end{proof}
