\problem{Tautology Proof}

This question contained a typo. I believe that the right hand side of the statement should be $((A \Rightarrow C) \wedge (B \Rightarrow C))$, but was $((A \Rightarrow C) \vee (B \Rightarrow C))$.

Prove that the following statement is a tautology:

$((A \vee B) \Rightarrow C) \Leftrightarrow ((A \Rightarrow C) \wedge (B \Rightarrow C))$

\solution

\part 

\begin{theorem}
$((A \vee B) \Rightarrow C) \Leftrightarrow ((A \Rightarrow C) \vee (B \Rightarrow C))$ is a tautology.
\end{theorem}

\begin{proof}
The left hand side $((A \vee B) \Rightarrow C)$ can be converted into $C \vee \neg (A \vee C)$ by rule nine (Absorption).
Then, this can be transformed using DeMorgan's law: $C \vee (\neg A \wedge \neg B)$. 
Further, by distributivity, the statement is broken apart: $(C \vee \neg A) \wedge (C \vee \neg B)$.
Each side of the statement can again be turned into an implication, resulting in $(A \Rightarrow C) \wedge (B \Rightarrow C)$. 
\end{proof}
